ver2_qbft_Style/Replica.dfy
@@ -5,6 +5,17 @@ module M_Replica {
     import opened M_SpecTypes
     import opened M_AuxilarilyFunc
 
+    /**
+     *  Bookeeping variables for a node
+     *  id : identifier
+     *  bc : local blockchain
+     *  c  : configuration about nodes and genesis block
+     *  viewNum : view number
+     *  prepareQC : Quorum Certificate for prepare message
+     *  commitQC : Qurum Certificate for commit message, also refers to "lockQC" at the HotStuff paper
+     *  msgRecieved : all the messages recieved
+     *  highestExecutedBlock : executed block with the highest view number
+     */
     datatype ReplicaState = ReplicaState(
         id : Address,
         bc : Blockchain,
@@ -12,35 +23,45 @@ module M_Replica {
         viewNum : nat,
         prepareQC : Cert,
         commitQC : Cert,
-        msgRecieved : set<Msg>
+        msgRecieved : set<Msg>,
+        highestExecutedBlock : Block
     )
 
+    /**
+     *  Replica Initialization
+     */
     predicate ReplicaInit(r : ReplicaState, id : Address, c : Configuration) 
     {
-        && r.c == c
-        && r.round == 0
-        && r.bc == [c.genesisBlock]
         && r.id == id
-        && r.prepareQC == None
-        && r.commitQC == None
+        && r.bc == [c.genesisBlock]
+        && r.c == c
+        && r.viewNum == 1
+        && r.prepareQC == CertNone
+        && r.commitQC == CertNone
+        && r.msgRecieved == {}
+        && r.highestExecutedBlock == EmptyBlock
     }
 
+    /**
+     *  All different transition states.
+     *  Current state (r) could transfer to the next state (r'), together with sending out some messages (outMsg)
+     */
     predicate ReplicaNext(r : ReplicaState, r' : ReplicaState, outMsg : set<MsgWithRecipient>)
     {
-        || UponNextView(r, r')
-        || UponPrepare(r, r')
-        || UponPreCommit(r, r')
-        || UponCommit(r, r')
-        || UponDecide(r, r')
-        || UponTimeOut(r, r')
+        || UponNextView(r, r', outMsg)
+        || UponPrepare(r, r', outMsg)
+        || UponPreCommit(r, r', outMsg)
+        || UponCommit(r, r', outMsg)
+        || UponDecide(r, r', outMsg)
+        || UponTimeOut(r, r', outMsg)
     }
 
     predicate UponNextView(r : ReplicaState, r' : ReplicaState, outMsg : set<MsgWithRecipient>)
     {
         var newLeader := leader(r.viewNum+1, r.c);
-        var newViewMsg := MsgWithRecipient(Msg(MT_NewView, None, r.prepareQC), leader);
+        var newViewMsg := MsgWithRecipient(Msg(MT_NewView, r.viewNum, EmptyBlock, r.prepareQC, SigNone), newLeader);
         && r' == r.(
-            viewNum := viewNum + 1
+            viewNum := r.viewNum + 1
         )
         && outMsg == {newViewMsg}
     }
@@ -53,7 +74,7 @@ module M_Replica {
             var matchMsgs := getMatchMsg(r.msgRecieved, MT_NewView, r.viewNum-1);
             var highQC := getHighQC(matchMsgs);
             var proposal := getNewBlock(highQC.node);
-            var proposeMsg := Msg(MT_Prepare, r.viewNum, proposal, highQC);
+            var proposeMsg := Msg(MT_Prepare, r.viewNum, proposal, highQC, SigNone);
 
             && r' == r.(msgRecieved := r.msgRecieved + {proposeMsg})
             && outMsg == Multicast(proposeMsg, r.c.nodes)
@@ -61,15 +82,15 @@ module M_Replica {
         else
             var matchMsgs := getMatchMsg(r.msgRecieved, MT_Prepare, r.viewNum);
             forall m | m in matchMsgs ::
-                var sig := Signature(r.Address, m.mType, m.viewNum, m.node);
-                var vote := Msg(MT_Prepare, r.viewNum, m.node, None, sig);
+                var sig := Signature(r.id, m.mType, m.viewNum, m.node);
+                var vote := Msg(MT_Prepare, r.viewNum, m.node, CertNone, sig);
                 var voteMsg := MsgWithRecipient(vote, leader);
                 if extension(m.node, m.justify.node)
-                    && safeNode(m.node, m.justify, r.lockedQC)
+                    && safeNode(m.node, m.justify, r.commitQC)
                 then
-                    vote in outMsg
+                    voteMsg in outMsg
                 else
-                    !(vote in outMsg)
+                    !(voteMsg in outMsg)
     }  
 
     predicate UponPreCommit(r : ReplicaState, r' : ReplicaState, outMsg : set<MsgWithRecipient>)
@@ -80,9 +101,11 @@ module M_Replica {
             var matchMsgs := getMatchMsg(r.msgRecieved, MT_Prepare, r.viewNum);
             if |matchMsgs| >= quorum(|r.c.nodes|)
             then
-                var signatures := v.partialSig | v in matchMsgs;
-                var prepareQc := Cert(MT_Prepare, matchMsgs[0].viewNum, matchMsgs[0].node, signatures);
-                var precommitMsg := Msg(MT_PreCommit, r.viewNum, None, prepareQC);
+                var m :| m in matchMsgs;
+                var sgns := ExtractSignatrues(matchMsgs);
+                // var signatures := m.partialSig;
+                var prepareQC := Cert(MT_Prepare, m.viewNum, m.node, sgns);
+                var precommitMsg := Msg(MT_PreCommit, r.viewNum, EmptyBlock, prepareQC, SigNone);
                 && r' == r.(msgRecieved := r.msgRecieved + {precommitMsg})
                 && outMsg == Multicast(precommitMsg, r.c.nodes)
             else
@@ -91,8 +114,8 @@ module M_Replica {
         else
             var matchQCs := getMatchQC(r.msgRecieved, MT_Prepare, r.viewNum);
             forall m | m in matchQCs ::
-                var sig := Signature(r.Address, m.mType, m.viewNum, m.node);
-                var vote := Msg(MT_PreCommit, r.viewNum, m.node, None, sig);
+                var sig := Signature(r.id, m.cType, m.viewNum, m.node);
+                var vote := Msg(MT_PreCommit, r.viewNum, m.node, CertNone, sig);
                 var voteMsg := MsgWithRecipient(vote, leader);
                 && r' == r.(prepareQC := m)
                 && voteMsg in outMsg
@@ -107,9 +130,10 @@ module M_Replica {
             var matchMsgs := getMatchMsg(r.msgRecieved, MT_PreCommit, r.viewNum);
             if |matchMsgs| >= quorum(|r.c.nodes|)
             then
-                var signatures := v.partialSig | v in matchMsgs;
-                var precommitQC := Cert(MT_PreCommit, matchMsgs[0].viewNum, matchMsgs[0].node, signatures);
-                var commitMsg := Msg(MT_Commit, r.viewNum, None, precommitQC);
+                var m :| m in matchMsgs;
+                var sgns := ExtractSignatrues(matchMsgs);
+                var precommitQC := Cert(MT_PreCommit, m.viewNum, m.node, sgns);
+                var commitMsg := Msg(MT_Commit, r.viewNum, EmptyBlock, precommitQC, SigNone);
                 && r' == r.(msgRecieved := r.msgRecieved + {commitMsg})
                 && outMsg == Multicast(commitMsg, r.c.nodes)
             else
@@ -118,10 +142,10 @@ module M_Replica {
         else
             var matchQCs := getMatchQC(r.msgRecieved, MT_PreCommit, r.viewNum);
             forall m | m in matchQCs ::
-                var sig := Signature(r.Address, m.mType, m.viewNum, m.node);
-                var vote := Msg(MT_Commit, r.viewNum, m.node, None, sig);
+                var sig := Signature(r.id, m.cType, m.viewNum, m.node);
+                var vote := Msg(MT_Commit, r.viewNum, m.node, CertNone, sig);
                 var voteMsg := MsgWithRecipient(vote, leader);
-                && r' == r.(lockedQC := m)
+                && r' == r.(commitQC := m)
                 && voteMsg in outMsg
     }
 
@@ -133,9 +157,10 @@ module M_Replica {
             var matchMsgs := getMatchMsg(r.msgRecieved, MT_Commit, r.viewNum);
             if |matchMsgs| >= quorum(|r.c.nodes|)
             then
-                var signatures := v.partialSig | v in matchMsgs;
-                var commitQC := Cert(MT_PreCommit, matchMsgs[0].viewNum, matchMsgs[0].node, signatures);
-                var decideMsg := Msg(MT_Decide, r.viewNum, None, commitQC);
+                var m :| m in matchMsgs;
+                var sgns := ExtractSignatrues(matchMsgs);
+                var commitQC := Cert(MT_PreCommit, m.viewNum, m.node, sgns);
+                var decideMsg := Msg(MT_Decide, r.viewNum, EmptyBlock, commitQC, SigNone);
                 && r' == r.(msgRecieved := r.msgRecieved + {decideMsg})
                 && outMsg == Multicast(decideMsg, r.c.nodes)
             else
@@ -145,7 +170,7 @@ module M_Replica {
             var matchQCs := getMatchQC(r.msgRecieved, MT_Commit, r.viewNum);
             forall m | m in matchQCs ::
                 && r' == r.(
-                    bc := r.bc + m.node
+                    bc := r.bc + [m.node]
                 )
     }
 
